%----------------------------------------------------------------------------------------
%   PACKAGES AND OTHER DOCUMENT CONFIGURATIONS
%----------------------------------------------------------------------------------------

\documentclass[11pt]{article}

\usepackage[english]{babel}
\usepackage[utf8x]{inputenc}
\usepackage{amsmath}
\usepackage{graphicx}
\usepackage{csquotes}
\usepackage{fancyvrb}
\usepackage{array}
\usepackage{relsize}
\usepackage[a4paper, total={6in, 8in}]{geometry}
\usepackage[colorinlistoftodos]{todonotes}

\setlength{\parindent}{0pt}

\newenvironment{conditions}
  {\par\vspace{\abovedisplayskip}\noindent\begin{tabular}{>{$}l<{$} @{${}={}$} l}}
  {\end{tabular}\par\vspace{\belowdisplayskip}}
\newcommand{\shortrnote}[1]{ &  & \text{\footnotesize\llap{#1}}}

%----------------------------------------------------------------------------------------
%   HEADING
%----------------------------------------------------------------------------------------

\newcommand{\BigO}[1]{\ensuremath{\operatorname{O}\left(#1\right)}}

\title{\textsc{Computational Finance}\\Coursework}
\author{Lawrence Jones \{lmj112\}}

\date{}
\begin{document}
\maketitle

%----------------------------------------------------------------------------------------
%   EXERCISE 1
%----------------------------------------------------------------------------------------

\subsection*{Exercise 1. Dividend Discount Model}

Assume that each stock of a company pays a dividend $D_t$ at the end of every
year, $t = 1, 2, 3, \ldots$, and denote by $r > 0$ the constant annual interest
rate (use yearly compounding).

\subsubsection*{Part (a)}

Computing the Net Present Value of the dividend stream:

\setcounter{equation}{0}
\begin{equation}
  \mathlarger{\mathlarger{\sum}}_{k=1}^{\infty}
    \frac{(1 + g)^{k}~D_{1}}{(1+r)^{k}}
\end{equation}
\
where:

\begin{conditions}
    D_{1}           & Initial dividend amount \\
    g               & Dividend growth rate \\
    r               & Constant annual interest rate
\end{conditions}

\setcounter{equation}{0}
\begin{eqnarray}
  &&= D_{1}\left(\sum_{k=1}^{\infty} \frac{\left(1+g\right)^{k-1}}{\left(1+r\right)^{k}}\right) \\
  &&= \frac{D_{1}}{\left(1+g\right)} \left(\sum_{k=1}^{\infty} \frac{\left(1+g\right)^{k}}{\left(1+r\right)^{k}}\right) \\
  &&= \frac{D_{1}}{\left(1+g\right)} \left(\sum_{k=0}^{\infty} \frac{\left(1+g\right)^{k}}{\left(1+r\right)^{k}} - 1\right) \\
  &&= \frac{D_{1}}{\left(1+g\right)} \left(\frac{1}{1 - \left(\frac{1+g}{1+r}\right)} - 1\right) \\
  &&= \frac{D_{1}}{\left(1+g\right)} \left(\frac{1+r}{r-g} - 1\right) \\
  &&= \frac{D_{1}}{\left(1+g\right)} \frac{1+g}{r-g} \\
  &&= \frac{D_{1}}{r-g}
\end{eqnarray}

\subsubsection*{Part (b)}

Find expression for\dots

\setcounter{equation}{0}
\begin{eqnarray}
  & \sum_{t=1}^{\infty} tx^{t} &= x + 2x^{2} + 3x^{3} + \dots \\
                               &&= \sum_{t=1}^{\infty} \left( \sum_{k=t}^{\infty} x^{k} \right) \\
                               &&= \sum_{t=1}^{\infty} \left( \frac{x^{t}}{1 - x} \right) \\
                               &&= \frac{\frac{x}{1 - x}}{1 - x} \\
                               &&= x\left(1 - x\right)^{-2}
\end{eqnarray}

The net present value of this dividend stream can be represented as\dots

\begin{eqnarray}
  & \sum_{t=1}^{\infty} \frac{\left(D_{1} - I\right) + tI}{\left(1 + r\right)^{t}} \
  &= \sum_{t=1}^{\infty} \frac{\left(D_{1} - I\right)}{\left(1+r\right)^{t}} + \sum_{t=1}^{\infty} \frac{tI}{\left(1+r\right)^{t}} \\
  &&= \left(D_{1} - I\right)\left( \sum_{t=0}^{\infty} \frac{1}{\left(1+r\right)^{t}} - 1 \right) + \dots \\
  &&= \left(D_{1} - I\right)\left( \frac{1}{1 - \left(\frac{1}{1+r}\right)} -1 \right) + \dots \\
  &&= \left(D_{1} - I\right)\left( \frac{r+1}{r} -1 \right) + \dots \\
  &&= \left( \frac{D_{1} - I}{r} \right) + \sum_{t=1}^{\infty} \frac{tI}{\left(1+r\right)^{t}} \\
  &&= \dots + I\left( \frac{1}{1+r} \left(1 - \frac{1}{1+r}\right)^{-2} \right) \\
  &&= \dots + I\left( \frac{1}{1+r} \left( \frac{1}{1 - \frac{1}{1+r}} \right)^{2} \right) \\
  &&= \left( \frac{D_{1} - I}{r} \right) + I\left( \frac{1+r}{r^{2}} \right) \\[4mm]
  &&= \frac{rD_{1} + I}{r^{2}}
\end{eqnarray}

\newpage

%----------------------------------------------------------------------------------------
%   EXERCISE 2
%----------------------------------------------------------------------------------------

\subsection*{Exercise 2. Fixed Income Securities}

Consider a 10\% coupon bond with a face value of £100 that matures in 2 years
from now. Assume that there is one coupon payment per year and that the bond is
absolutely risk free.

\subsubsection*{Part (a)}

The cash flow stream with spot rates is computed in the following table.

\begin{center}
  \begin{tabular}{| l | l | l | l |}
    \hline
    \textbf{Year}           & 1     & 2     & 3      \\ \hline
    \textbf{Spot Rate}      & 4\%   & 6\%   & 8\%    \\ \hline
    \textbf{Discount}       & 0.962 & 0.890 & 0.794  \\ \hline
    \textbf{Cash Flow}      & 10    & 110   & 0      \\ \hline
    \textbf{Present Value}  & 9.62  & 97.90 & 0      \\ \hline
  \end{tabular}
\end{center}

The price of the bond is the sum of the present values\dots

\[\sum_{t=1}^{2} PV_{t} = 9.62 + 97.90 + 0 = £107.52\]

\subsubsection*{Part (b)}

From our definition of Yield to Maturity with yearly coupon payments\dots

\setcounter{equation}{0}
\begin{equation}
P = \frac{F}{\left(1 + \lambda\right)^{n}} + \sum_{k=1}^{n} \frac{C}{\left(1 + \lambda\right)^{k}}
\end{equation}
\
where:

\begin{conditions}
  P               & Bond price (market value) \\
  F               & Face value \\
  n               & Years until maturity \\
  \lambda         & Yield to Maturity \\
  C               & Coupon amount (coupon rate * face value)
\end{conditions}

\begin{eqnarray}
  & P \
\
  &= \frac{F}{\left(1 + \lambda\right)^{2}} + \frac{C}{1 + \lambda} + \frac{C}{\left(1 + \lambda\right)^{2}} \\
  &&= \frac{F + C}{\left(1 + \lambda\right)^{2}} + \frac{C\left(1 + \lambda\right)}{\left(1 + \lambda\right)^{2}} \\
  &&= \frac{F + 2C + C\lambda}{\left(1 + \lambda\right)^{2}} \\
\end{eqnarray}

Rearranging for a $\lambda$ quadratic gives\dots

\[P\lambda^{2} + \left(2P - C\right)\lambda + \left(P - F - 2C\right) = 0\]

Using quadratic formula\dots

\begin{eqnarray}
  & \lambda &= \frac{ -\left(2P - C\right) \pm \sqrt{\left(2P - C\right)^{2} - 4P\left(P - F - 2C\right)} }{2P} \\
  &&= \frac{ C - 2P \pm \sqrt{C^{2} + 4CP + 4FP} }{2P}
\end{eqnarray}

For this bond\dots

\[ \lambda = -1.966 \text{~or~} 0.059 \]

Yield is positive, so the yield value is 5.9\%.

\subsubsection*{Part (c)}

Definition of Macaulay duration\dots

\[ D = \frac{PV[t_{0}]t_{0} + \dots + PV[t_{n}]t_{n}}{PV[t_{0}] + \dots + PV[t_{n}]} \]
\
where:

\begin{conditions}
  D               & Macaulay duration \\
  t_{i}           & Time in years \\
  PV[t_{i}]       & Present value of cash flow at time $t_{i}$ wrt. yield
\end{conditions}

So for this bond\dots

\setcounter{equation}{0}
\begin{eqnarray}
  & D &= \frac{PV[t_{0}]t_{0} + PV[t_{1}]t_{1} + PV[t_{2}]t_{2}}{PV[t_{0}] + PV[t_{1}] + PV[t_{2}]} \\
  &&= \frac{0 + 9.44 + 2*98.08}{0 + 9.44 + 98.08} \\
  &&= \text{1.91 years}
\end{eqnarray}

\subsubsection*{Part (d)}

First we are required to compute the spot rate from the next year. Due to expectation dynamics,
we know that the spot rates to come can be calculated from todays forward rates.

\[ s' = f_{1,2}, f_{1,3}, \dots \]

We have the definition for a forward rate between time i and j\dots

\[ f_{i,j} = \left[ \frac{\left(1 + s_{j}\right)^{j}}{\left(1 + s_{i}\right)^{i}} \right]^{\frac{1}{j - i}} - 1 \]

So we must use this to define $s'$\dots

\begin{eqnarray}
  & s'_{1} = f_{1,2} &= \left[ \frac{\left(1 + 0.06\right)^{2}}{1.04} \right]^{\frac{1}{1}} - 1 = 8.04\% \\
  & s'_{2} = f_{1,3} &= \left[ \frac{\left(1 + 0.08\right)^{3}}{1.04} \right]^{\frac{1}{2}} - 1 = 10.06\%
\end{eqnarray}

We can now calculate the price of the bond in a years time, noting that the first coupon payment is still due\dots

\[ P = \left(10 / 1\right) + \left(110 / 1.0804\right) = £111.81 \]
\\
From this we can now compute Yield to Maturity\dots

\begin{eqnarray}
  & P &= \frac{F}{\left(1 + \lambda\right)^{n}} + \sum_{k=0}^{n} \frac{C}{\left(1 + \lambda\right)^{k}} \\[4mm]
  &&= \frac{F}{\left(1 + \lambda\right)^{1}} + \frac{C}{\left(1 + \lambda\right)^{0}} + \frac{C}{\left(1 + \lambda\right)^{1}} \\[4mm]
  &&= \frac{F + C}{1 + \lambda} + C \\[4mm]
  & \lambda &= \frac{F + C}{P - C} - 1 \\[4mm]
  &&= 8.04\%
\end{eqnarray}

\newpage

%----------------------------------------------------------------------------------------
%   EXERCISE 3
%----------------------------------------------------------------------------------------

\subsection*{Exercise 3. Portfolio Optimisation}

Consider a market that contains $n$ risky assets and one risk-free asset. Denote by
$\bar{r}=\left(\bar{r}_{1},\dots,\bar{r}_{n}\right)$ the vector of expected returns and by

\begin{equation*}
\Sigma = \begin{pmatrix}
  cov(r_{1},r_{2}) & \dots  & cov(r_{1},r_{n}) \\
  \vdots           & \ddots & \vdots \\
  cov(r_{n},r_{1}) & \dots  & cov(r_{n},r_{n})
\end{pmatrix}
\end{equation*}

the covariance matric of the risky assets, respectively. Moreover, let $r_{f}$ be the risk-free
rate of return. Assume that $\Sigma$ is strictly positive definite and therefore invertible.

\subsubsection*{Part (a)}

\textit{What is the expected return $\bar{r}_{P}$ and the variance $\sigma^{2}_{P}$ of a
  portfolio that assigns weights $\textbf{w} = (w_{i},\dots,w_{n})$ to the risky assets and
weight $w_{0}$ to the risk-free assets?} \\

Expected return is\dots

\setcounter{equation}{0}
\begin{eqnarray}
  & \bar{r}_{P} &= w_{0}r_{f} + E\left[\sum_{i=1}^{n} w_{i}r_{i}\right] \\
  &&= w_{0}r_{f} + \sum_{i=1}^{n} w_{i} E\left[r_{i}\right] \\
  &&= w_{0}r_{f} + \sum_{i=1}^{n} w_{i} \bar{r}_{i}
\end{eqnarray}

Risk free assets have no variance, and so the variance of our portfolio can be expressed
in terms of our risky weights only\dots

\[ \sigma^{2}_{P} = \sum_{i,j=1}^{n} w_{i}\sigma_{ij}w_{j} \]

\subsubsection*{Part (b)}

\textit{We wish to maximise $\bar{r}_{P} - \frac{a}{2}\sigma^{2}_{P}$, where $a
> 0$ can be viewed as a risk aversion parameter. Formulate this as a quadratic
program without constraints.} \\

As $a > 0$, then we know that to maximise this equation we must minimise $\frac{a}{2}\sigma^{2}_{P}$.
This can be represented as a quadratic program as\dots

\begin{center}
  \begin{tabular}{ l l r }
    \textbf{Minimize}   & $\frac{a}{2} \sigma^{2}_{P}$ & \textit{variance} \\[8mm]
    \textbf{Subject to} & $w_{0}r_{f} + \sum_{i=1}^{n} w_{i}\bar{r}_{i} = \bar{r}_{P}$ & \textit{return} \\[2mm]
                        & $w_{0} + \sum_{i=1}^{n} w_{i} = 1$ & \textit{budget} \\[4mm]
  \end{tabular}
\end{center}

We can reform this as a Lagrangian function in order to remove constraints\dots

\begin{eqnarray}
  & L(w_{i},\lambda,\mu) &= \frac{a}{2}\sigma^{2}_{P} - \lambda\left(w_{0}r_{f} + \sum_{i=1}^{n} w_{i}\bar{r}_{i} - \bar{r}_{P}\right) - \mu\left(w_{0} + \sum_{i=1}^{n} w_{i} - 1\right) \\
  &&= \frac{a}{2}\sigma^{2}_{P} - \
  \lambda\left( \sum_{i=1}^{n}{w_{i}\left(\bar{r}_{i} - r_{f}\right)} + r_{f} - r_{P} \right) - \
  \mu\left(w_{0} + \sum_{i=1}^{n} w_{i} - 1\right)
\end{eqnarray}

\subsubsection*{Part (c)}

Differentiating the Lagrangian yields optimality conditions for Part (b)

\begin{eqnarray}
  & \frac{\delta L}{\delta w_{i}} &: a\sum_{j=1}^{n} \sigma_{ij}w_{i} - \lambda\left(\bar{r}_{i} - r_{f}\right) - \mu = 0 \\
  & \frac{\delta L}{\delta \lambda} &: \sum_{i=1}^{n}w_{i}\left(\bar{r}_{i} - r_{f}\right) + r_{f} = r_{P} \\
  & \frac{\delta L}{\delta \mu} &: w_{0} + \sum_{i=1}^{n} w_{i} = 1
\end{eqnarray}

\newpage

%----------------------------------------------------------------------------------------
%   EXERCISE 4
%----------------------------------------------------------------------------------------

\subsection*{Exercise 4. Fixed Income Securities}

Assume a constant ideal bank with yearly interest of 6\%, compounded monthly. Consider an
annuity that pays £100 monthly over a period of ten years; compute the size of a single cash
flow arising after five years that is equivalent to the annuity.

\subsubsection*{Part (a)}

We calculate the annuity present value as the sum of all the payments at the discount factor
for the time they are received\dots

\setcounter{equation}{0}
\begin{eqnarray}
  & PV[annuity] &= \sum_{t=1}^{10 \times 12} \frac{100}{\left(1 + \frac{0.06}{12}\right)^{t}} \\[4mm]
  &&= 100 \left[ \frac{\left(1 - 1.005^{-120}\right)}{1.005\left(1 - 1.005^{-1}\right)} \right] \\[4mm]
  &&= £9,007.35
\end{eqnarray}

A cash flow stream of equivalent value is one that has an equivalent present value. We must find
the amount ($a$) of the single payment which when discounted for five years of compounded interest
is equivalent to the present value of the annuity\dots

\begin{eqnarray}
  & PV[annuity] &= \frac{a}{\left(1 + \frac{0.06}{12}\right)^{5 \times 12}} \\[4mm]
  & a &= PV[annuity] \times 1.005^{60} \\[4mm]
      &&= £12,149.57
\end{eqnarray}

\subsubsection*{Part (b)}

If we have spot rate $s_{k}$ associated with maturity $k$, then we can compute our forward
rate using the following formula\dots

\[ f_{i,j} = \left[ \frac{\left(1 + s_{j}\right)^{j}}{\left(1 + s_{i}\right)^{i}} \right]^{\frac{1}{j-i}} -1 \]
\\
But if we know that $\forall k\in\mathbb{N}:s_{k} = r$, then we can simply this\dots

\setcounter{equation}{0}
\begin{eqnarray}
  & f_{i,j} &= \left[ \frac{\left(1+r\right)^{j}}{\left(1+r\right)^{i}} \right]^{\frac{1}{j-i}} -1 \\[3mm]
  &&= \left[ \left(1+r\right)^{j-i} \right]^{\frac{1}{j-i}} -1 \\[3mm]
  &&= \left(1+r\right)^{1} -1 \\[3mm]
  &&= r
\end{eqnarray}

\subsubsection*{Part (c)}

\textit{A corporation issues a 10\%, 20-year bond at a time when yields are 10\%. The
bond has a call provision that allows the corporation to force a bond holder to
redeem his or her bond at face value plus 5\%. After 5 years the corporation
finds that exercise of this call provision is advantageous.}\\

For calling the bond to be advantageous to the corporation, the money the corporation
would have to pay ($1.05 \times F$) at the five year mark would have to be worth less
than the present value of the remaining bond coupon payments plus the final face value
payment on maturity.

\[ 1.05 \times F < \frac{F}{\left(1+\lambda\right)^{15}} + \frac{cF}{\lambda}\left[1 - \frac{1}{\left(1+\lambda\right)^{15}}\right] \] \\

What is clear from this equation is that the inequality is not affected by the face
value. This is to be expected, as the answer to whether this is advantageous depends
fundamentally on the ratio between yield and multiplier of the face value to repay,
not the size of the face value.

\[ 1.05 < \frac{1}{\left(1+\lambda\right)^{15}} + \frac{c}{\lambda}\left[1 - \frac{1}{\left(1+\lambda\right)^{15}}\right] \] \\

Solving for $\lambda$ would require expanding $(1 + \lambda)^{15}$ which gets
messy by hand. Using a solver to find the result, we can determine that
$\lambda = 9.37\%$, a value that is consistent with the expectation that yield
must have decreased; the cost of supporting the bond had increased beyond the
cost of recalling it now.

\newpage

%----------------------------------------------------------------------------------------
%   EXERCISE 5
%----------------------------------------------------------------------------------------

\subsection*{Exercise 5. Mean-Variance Portfolio Theory}

\subsubsection*{Part (a)}

The total return of our stock, $R$, is defined as\dots

\[ R_{stock} = \frac{X_{1}}{X_{0}} \]

We can see from this equation that as the sale price $X_{1}$ increases, then so does return.
The total return on our short can be calculated as the ratio between the money received at
liquidity and the money invested up front. \\

The initial investment is the deposit of amount $X_{0}$, and then on liquidity we receive
the difference in sale price $X_{0} - X_{1}$ as our profit and our initial deposit returned.

\setcounter{equation}{0}
\begin{eqnarray}
  & R_{short} &= \frac{X_{0} + \left(X_{0} - X_{1}\right)}{X_{0}} \\
  &&= \frac{2X_{0} - X_{1}}{X_{0}} \\
  &&= 2 - \frac{X_{1}}{X_{0}} \\
  &&= 2 - R_{stock}
\end{eqnarray}

\subsubsection*{Part (b)}

We can compute the variance of a portfolio with

\[ var = \sigma^{2}_{P} = \sum_{i,j=1}^{n} w_{i} \sigma_{ij} w_{j} \] \\

and so with our two stocks, we can compute the variance to be\dots

\begin{eqnarray}
  & \sigma^{2}_{P} &= \sum_{i,j=1}^{2} w_{i} \sigma_{ij} w_{j} \\
  &&= w_{1}^{2}\sigma^{2}_{1} + 2w_{1}w_{2}\sigma_{12} + w_{2}^{2}\sigma^{2}_{2}
\end{eqnarray}\\[1mm]
\
We can minimise the variance by expressing this problem as a Lagrangian, with the constraint
of $\sum_{i=1}^{n} w_{i} = 1$.

\begin{eqnarray}
  & L(w_{1},w_{2},\lambda) &= w_{1}^{2}\sigma^{2}_{1} + 2w_{1}w_{2}\sigma_{12} + w_{2}^{2}\sigma^{2}_{2} \
  - \lambda\left(w_{1} + w_{2} - 1\right)
\end{eqnarray}

We can now establish the optimality conditions by differentiating the Lagrange\dots

\begin{eqnarray}
  & \frac{\delta L}{\delta w_{1}} &: 2w_{1}\sigma^{2}_{1} + 2w_{2}\sigma_{12} - \lambda = 0 \label{eq:5b1}\\
  & \frac{\delta L}{\delta w_{2}} &: 2w_{2}\sigma^{2}_{2} + 2w_{1}\sigma_{12} - \lambda = 0 \label{eq:5b2}\\
  & \frac{\delta L}{\delta \lambda} &: w_{1} + w_{2} = 1
\end{eqnarray}

Calculating $\left(\ref{eq:5b1}\right) - \left(\ref{eq:5b2}\right)$ gives\dots

\begin{eqnarray}
  & 0 &= 2w_{1}\sigma^{2}_{1} + 2w_{2}\sigma_{12} - 2w_{2}\sigma^{2}_{2} - 2w_{1}\sigma_{12} \\
  &&= w_{1}\sigma^{2}_{1} + \left(1-w_{1}\right)\sigma_{12} - \left(1-w_{1}\right)\sigma_{2}^{2} - w_{1}\sigma_{12} \\
  &&= w_{1}\left(\sigma^{2}_{1} - 2\sigma_{12} + \sigma^{2}_{2}\right) - \sigma^{2}_{2} + \sigma_{12} \\
  & w_{1} &= \frac{\sigma^{2}_{2} - \sigma_{12}}{\sigma^{2}_{1} - 2\sigma_{12} + \sigma^{2}_{2}}
\end{eqnarray}\\[1mm]
\
Similarly, $w_{2}$ can be computed as\dots

\[ w_{2} = \frac{\sigma^{2}_{1} - \sigma_{12}}{\sigma^{2}_{1} - 2\sigma_{12} + \sigma^{2}_{2}} \] \\

The mean rate of return can be defined in terms of $w_{1}$ and $w_{2}$\dots

\[ \bar{r} = w_{1}\bar{r}_{1} + w_{2}\bar{r}_{2} \]

\end{document}
